Launchbury/FTreeImplCardinality.thy
@@ -14,18 +14,21 @@ fun unstack :: "stack \<Rightarrow> exp \<Rightarrow> exp" where
 | "unstack (Arg x # S) e = unstack S (App e x)"
 | "unstack (Dummy x # S) e = unstack S e"
 
-fun Fstack :: "stack \<Rightarrow> var ftree"
-  where "Fstack [] = \<bottom>"
-  | "Fstack (Alts e1 e2 # S) = Fstack S"
-  | "Fstack (Upd x # S) = Fstack S"
-  | "Fstack (Arg x # S) = many_calls x \<otimes>\<otimes> Fstack S"
-  | "Fstack (Dummy x # S) = Fstack S"
+fun Fstack :: "Arity list \<Rightarrow> stack \<Rightarrow> var ftree"
+  where "Fstack _ [] = \<bottom>"
+  | "Fstack (a#as) (Alts e1 e2 # S) = (Fexp e1\<cdot>a \<oplus>\<oplus> Fexp e2\<cdot>a) \<otimes>\<otimes> Fstack as S"
+  | "Fstack as (Arg x # S) = many_calls x \<otimes>\<otimes> Fstack as S"
+  | "Fstack as (_ # S) = Fstack as S"
 
+
+
+(*
 lemma carrier_Fstack[simp]: "carrier (Fstack S) = ap S"
   by (induction S rule: Fstack.induct) (auto simp add: empty_is_bottom[symmetric])
+*)
 
-fun prognosis :: "AEnv \<Rightarrow> Arity \<Rightarrow> conf \<Rightarrow> var \<Rightarrow> two"
-   where "prognosis ae a (\<Gamma>, e, S) = pathsCard (paths (substitute (FBinds \<Gamma>\<cdot>ae) (thunks \<Gamma>) (Fexp e\<cdot>a \<otimes>\<otimes> Fstack S)))"
+fun prognosis :: "AEnv \<Rightarrow> Arity list \<Rightarrow> Arity \<Rightarrow> conf \<Rightarrow> var \<Rightarrow> two"
+   where "prognosis ae as a (\<Gamma>, e, S) = pathsCard (paths (substitute (FBinds \<Gamma>\<cdot>ae) (thunks \<Gamma>) (Fexp e\<cdot>a \<otimes>\<otimes> Fstack as S)))"
 end
 
 end
