Launchbury/CardinalityAnalysisSig.thy
@@ -3,7 +3,7 @@ imports Arity AEnv "Cardinality-Domain" SestoftConf
 begin
 
 locale CardinalityPrognosis = 
-  fixes prognosis :: "AEnv \<Rightarrow> Arity \<Rightarrow> conf \<Rightarrow> (var \<Rightarrow> two)"
+  fixes prognosis :: "AEnv \<Rightarrow> Arity list \<Rightarrow> Arity \<Rightarrow> conf \<Rightarrow> (var \<Rightarrow> two)"
 
 locale CardinalityHeap = 
   fixes cHeap :: "heap \<Rightarrow> exp \<Rightarrow> Arity \<rightarrow> (var \<Rightarrow> two)"
