Launchbury/FTreeImplCardinalityCorrect.thy
@@ -20,6 +20,10 @@ lemma const_on_edom_disj: "const_on f S empty \<longleftrightarrow> edom f \<int
 
 context FTreeAnalysisCarrier
 begin
+  lemma carrier_Fstack: "carrier (Fstack as S) \<subseteq> fv S"
+    by (induction S rule: Fstack.induct)
+       (auto simp add: empty_is_bottom[symmetric] carrier_Fexp dest!: set_mp[OF Aexp_edom])
+
   lemma carrier_FBinds: "carrier ((FBinds \<Gamma>\<cdot>ae) x) \<subseteq> fv \<Gamma>"
   apply (simp add: Fexp.AnalBinds_lookup)
   apply (auto split: option.split simp add: empty_is_bottom[symmetric] )
@@ -33,125 +37,119 @@ begin
 
   sublocale CardinalityPrognosisShape prognosis
   proof
-    fix \<Gamma> :: heap and ae ae' :: AEnv and u e S
+    fix \<Gamma> :: heap and ae ae' :: AEnv and u e S as
     assume "ae f|` domA \<Gamma> = ae' f|` domA \<Gamma>"
     from Fexp.AnalBinds_cong[OF this]
-    show "prognosis ae u (\<Gamma>, e, S) = prognosis ae' u (\<Gamma>, e, S)" by simp
+    show "prognosis ae as u (\<Gamma>, e, S) = prognosis ae' as u (\<Gamma>, e, S)" by simp
   next
-    fix ae a \<Gamma> e S
-    show "const_on (prognosis ae a (\<Gamma>, e, S)) (ap S) many"
+    fix ae as a \<Gamma> e S
+    show "const_on (prognosis ae as a (\<Gamma>, e, S)) (ap S) many"
     proof
       fix x
       assume "x \<in> ap S"
-      hence "[x,x] \<in> paths (Fstack S)"
+      hence "[x,x] \<in> paths (Fstack as S)"
         by (induction S rule: Fstack.induct)
            (auto 4 4 intro: set_mp[OF both_contains_arg1] set_mp[OF both_contains_arg2] paths_Cons_nxt)
-      hence "[x,x] \<in> paths (Fexp e\<cdot>a \<otimes>\<otimes> Fstack S)"
+      hence "[x,x] \<in> paths (Fexp e\<cdot>a \<otimes>\<otimes> Fstack as S)"
         by (rule set_mp[OF both_contains_arg2])
-      hence "[x,x] \<in> paths (substitute (FBinds \<Gamma>\<cdot>ae) (thunks \<Gamma>) (Fexp e\<cdot>a \<otimes>\<otimes> Fstack S))" 
+      hence "[x,x] \<in> paths (substitute (FBinds \<Gamma>\<cdot>ae) (thunks \<Gamma>) (Fexp e\<cdot>a \<otimes>\<otimes> Fstack as S))" 
         by (rule set_mp[OF substitute_contains_arg])
-      hence "pathCard [x,x] x \<sqsubseteq> pathsCard (paths (substitute (FBinds \<Gamma>\<cdot>ae) (thunks \<Gamma>) (Fexp e\<cdot>a \<otimes>\<otimes> Fstack S))) x"
+      hence "pathCard [x,x] x \<sqsubseteq> pathsCard (paths (substitute (FBinds \<Gamma>\<cdot>ae) (thunks \<Gamma>) (Fexp e\<cdot>a \<otimes>\<otimes> Fstack as S))) x"
         by (metis fun_belowD paths_Card_above)
       also have "pathCard [x,x] x = many"  by (auto simp add: pathCard_def)
       finally
-      show "prognosis ae a (\<Gamma>, e, S) x = many"
+      show "prognosis ae as a (\<Gamma>, e, S) x = many"
         by (auto intro: below_antisym)
     qed
   next
-    fix \<Gamma> \<Delta> :: heap and e :: exp and ae :: AEnv and u S
+    fix \<Gamma> \<Delta> :: heap and e :: exp and ae :: AEnv and as u S
     assume "map_of \<Gamma> = map_of \<Delta>"
     hence "FBinds \<Gamma> = FBinds \<Delta>" and "thunks \<Gamma> = thunks \<Delta>" by (auto intro!: cfun_eqI  thunks_cong simp add: Fexp.AnalBinds_lookup)
-    thus "prognosis ae u (\<Gamma>, e, S) = prognosis ae u (\<Delta>, e, S)"  by simp
+    thus "prognosis ae as u (\<Gamma>, e, S) = prognosis ae as u (\<Delta>, e, S)"  by simp
   next
-    fix \<Gamma> :: heap and e :: exp and ae :: AEnv and u S x
-
-    show "prognosis ae u (delete x \<Gamma>, e, S) \<sqsubseteq> prognosis ae u (\<Gamma>, e, S)"
-      by (simp add: substitute_T_delete empty_is_bottom)
-         (intro pathsCard_mono' paths_mono substitute_mono1' Fexp.AnalBinds_delete_below)
+    fix \<Gamma> :: heap and e :: exp and ae :: AEnv and as u S x
+    show "prognosis ae as u (\<Gamma>, e, S) \<sqsubseteq> prognosis ae as u (\<Gamma>, e, Upd x # S)" by simp
   next
-    fix \<Gamma> :: heap and e :: exp and ae :: AEnv and u S x
-    show "prognosis ae u (\<Gamma>, e, S) \<sqsubseteq> prognosis ae u (\<Gamma>, e, Upd x # S)" by simp
-  next
-  fix \<Gamma> :: heap and e :: exp and ae :: AEnv and a S x
+  fix \<Gamma> :: heap and e :: exp and ae :: AEnv and as a S x
   assume "ae x = \<bottom>"
 
   hence "FBinds (delete x \<Gamma>)\<cdot>ae = FBinds \<Gamma>\<cdot>ae" by (rule Fexp.AnalBinds_delete_bot)
   moreover
   hence "((FBinds \<Gamma>\<cdot>ae) x) = \<bottom>" by (metis Fexp.AnalBinds_delete_lookup)
   ultimately
-  show "prognosis ae a (\<Gamma>, e, S) \<sqsubseteq> prognosis ae a (delete x \<Gamma>, e, S)"
+  show "prognosis ae as a (\<Gamma>, e, S) \<sqsubseteq> prognosis ae as a (delete x \<Gamma>, e, S)"
     by (simp add: substitute_T_delete empty_is_bottom)
   next
-    fix ae a \<Gamma> x S
+    fix ae as a \<Gamma> x S
     have "once \<sqsubseteq> (pathCard [x]) x" by (simp add: two_add_simp)
     also have "pathCard [x] \<sqsubseteq> pathsCard ({[],[x]})"
       by (rule paths_Card_above) simp
     also have "\<dots> = pathsCard (paths (single x))" by simp
     also have "single x \<sqsubseteq> (Fexp (Var x)\<cdot>a)" by (rule Fexp_Var)
-    also have "\<dots> \<sqsubseteq> Fexp (Var x)\<cdot>a \<otimes>\<otimes> Fstack S" by (rule both_above_arg1)
-    also have "\<dots> \<sqsubseteq> substitute  (FBinds \<Gamma>\<cdot>ae) (thunks \<Gamma>) (Fexp (Var x)\<cdot>a \<otimes>\<otimes> Fstack S)" by (rule substitute_above_arg)
-    also have "pathsCard (paths \<dots>) x =  prognosis ae a (\<Gamma>, Var x, S) x" by simp
+    also have "\<dots> \<sqsubseteq> Fexp (Var x)\<cdot>a \<otimes>\<otimes> Fstack as S" by (rule both_above_arg1)
+    also have "\<dots> \<sqsubseteq> substitute  (FBinds \<Gamma>\<cdot>ae) (thunks \<Gamma>) (Fexp (Var x)\<cdot>a \<otimes>\<otimes> Fstack as S)" by (rule substitute_above_arg)
+    also have "pathsCard (paths \<dots>) x = prognosis ae as a (\<Gamma>, Var x, S) x" by simp
     finally
-    show "once \<sqsubseteq> prognosis ae a (\<Gamma>, Var x, S) x"
+    show "once \<sqsubseteq> prognosis ae as a (\<Gamma>, Var x, S) x"
       by this (rule cont2cont_fun, intro cont2cont)+
   qed
 
   sublocale CardinalityPrognosisApp prognosis
   proof default
-    fix ae a \<Gamma> e x S
-    have "Fexp e\<cdot>(inc\<cdot>a)  \<otimes>\<otimes> many_calls x \<otimes>\<otimes> Fstack S = many_calls x  \<otimes>\<otimes> (Fexp e)\<cdot>(inc\<cdot>a) \<otimes>\<otimes> Fstack S"
+    fix ae as a \<Gamma> e x S
+    have "Fexp e\<cdot>(inc\<cdot>a)  \<otimes>\<otimes> many_calls x \<otimes>\<otimes> Fstack as S = many_calls x  \<otimes>\<otimes> (Fexp e)\<cdot>(inc\<cdot>a) \<otimes>\<otimes> Fstack as S"
       by (metis both_assoc both_comm)
-    thus "prognosis ae (inc\<cdot>a) (\<Gamma>, e, Arg x # S) \<sqsubseteq> prognosis ae a (\<Gamma>, App e x, S)"
+    thus "prognosis ae as (inc\<cdot>a) (\<Gamma>, e, Arg x # S) \<sqsubseteq> prognosis ae as a (\<Gamma>, App e x, S)"
       by simp (intro pathsCard_mono' paths_mono substitute_mono2' both_mono1' Fexp_App)
   qed
 
   sublocale CardinalityPrognosisLam prognosis
   proof default
-    fix ae a \<Gamma> e y x S
+    fix ae as a \<Gamma> e y x S
     have "Fexp e[y::=x]\<cdot>(pred\<cdot>a) \<sqsubseteq> many_calls x  \<otimes>\<otimes> Fexp (Lam [y]. e)\<cdot>a"
       by (rule below_trans[OF Fexp_subst both_mono2'[OF Fexp_Lam]])
-    moreover have "Fexp (Lam [y]. e)\<cdot>a \<otimes>\<otimes> many_calls x \<otimes>\<otimes> Fstack S = many_calls x  \<otimes>\<otimes> Fexp (Lam [y]. e)\<cdot>a \<otimes>\<otimes> Fstack S"
+    moreover have "Fexp (Lam [y]. e)\<cdot>a \<otimes>\<otimes> many_calls x \<otimes>\<otimes> Fstack as S = many_calls x  \<otimes>\<otimes> Fexp (Lam [y]. e)\<cdot>a \<otimes>\<otimes> Fstack as S"
       by (metis both_assoc both_comm)
     ultimately  
-    show "prognosis ae (pred\<cdot>a) (\<Gamma>, e[y::=x], S) \<sqsubseteq> prognosis ae a (\<Gamma>, Lam [y]. e, Arg x # S)"
+    show "prognosis ae as (pred\<cdot>a) (\<Gamma>, e[y::=x], S) \<sqsubseteq> prognosis ae as a (\<Gamma>, Lam [y]. e, Arg x # S)"
       by simp (intro pathsCard_mono' paths_mono substitute_mono2' both_mono1')
   qed
 
   sublocale CardinalityPrognosisVar prognosis
   proof default
-    fix \<Gamma> :: heap and e :: exp and x :: var and ae :: AEnv and u a S
+    fix \<Gamma> :: heap and e :: exp and x :: var and ae :: AEnv and as u a S
     assume "map_of \<Gamma> x = Some e"
     assume "ae x = up\<cdot>u"
 
-    have "pathsCard (paths (substitute (FBinds \<Gamma>\<cdot>ae) (thunks \<Gamma>) (Fexp e\<cdot>u \<otimes>\<otimes> Fstack S))) = pathsCard (paths (nxt (and_then x (substitute (FBinds \<Gamma>\<cdot>ae) (thunks \<Gamma>) (Fexp e\<cdot>u  \<otimes>\<otimes> Fstack S))) x))"
+    have "pathsCard (paths (substitute (FBinds \<Gamma>\<cdot>ae) (thunks \<Gamma>) (Fexp e\<cdot>u \<otimes>\<otimes> Fstack as S))) = pathsCard (paths (nxt (and_then x (substitute (FBinds \<Gamma>\<cdot>ae) (thunks \<Gamma>) (Fexp e\<cdot>u  \<otimes>\<otimes> Fstack as S))) x))"
       by simp
     also
-    have "\<dots> \<sqsubseteq> record_call x\<cdot>(pathsCard (paths (and_then x (substitute (FBinds \<Gamma>\<cdot>ae) (thunks \<Gamma>) (Fexp e\<cdot>u  \<otimes>\<otimes> Fstack S)))))"
+    have "\<dots> \<sqsubseteq> record_call x\<cdot>(pathsCard (paths (and_then x (substitute (FBinds \<Gamma>\<cdot>ae) (thunks \<Gamma>) (Fexp e\<cdot>u  \<otimes>\<otimes> Fstack as S)))))"
       by (rule pathsCard_paths_nxt)
     also
-    have "\<dots> = record_call x\<cdot>(pathsCard (paths (and_then x (substitute (FBinds \<Gamma>\<cdot>ae) (thunks \<Gamma>) (Fstack S  \<otimes>\<otimes> Fexp e\<cdot>u)))))"
+    have "\<dots> = record_call x\<cdot>(pathsCard (paths (and_then x (substitute (FBinds \<Gamma>\<cdot>ae) (thunks \<Gamma>) (Fstack as S \<otimes>\<otimes> Fexp e\<cdot>u)))))"
       by (metis both_comm)
     also
-    have "\<dots> = record_call x\<cdot>(pathsCard (paths (and_then x (substitute (FBinds \<Gamma>\<cdot>ae) (thunks \<Gamma>) (Fstack S  \<otimes>\<otimes> (FBinds \<Gamma>\<cdot>ae) x)))))"
+    have "\<dots> = record_call x\<cdot>(pathsCard (paths (and_then x (substitute (FBinds \<Gamma>\<cdot>ae) (thunks \<Gamma>) (Fstack as S \<otimes>\<otimes> (FBinds \<Gamma>\<cdot>ae) x)))))"
       using `map_of \<Gamma> x = Some e` `ae x = up\<cdot>u` by (simp add: Fexp.AnalBinds_lookup)
     also
     assume "isVal e"
     hence "x \<notin> thunks \<Gamma>" using `map_of \<Gamma> x = Some e` by (metis thunksE)
     hence "FBinds \<Gamma>\<cdot>ae = f_nxt (FBinds \<Gamma>\<cdot>ae) (thunks \<Gamma>) x" by (auto simp add: f_nxt_def)
-    hence "and_then x (substitute (FBinds \<Gamma>\<cdot>ae) (thunks \<Gamma>) (Fstack S  \<otimes>\<otimes> (FBinds \<Gamma>\<cdot>ae) x)) = substitute (FBinds \<Gamma>\<cdot>ae) (thunks \<Gamma>) (and_then x (Fstack S))"
+    hence "and_then x (substitute (FBinds \<Gamma>\<cdot>ae) (thunks \<Gamma>) (Fstack as S \<otimes>\<otimes> (FBinds \<Gamma>\<cdot>ae) x)) = substitute (FBinds \<Gamma>\<cdot>ae) (thunks \<Gamma>) (and_then x (Fstack as S))"
       by (simp add: substitute_and_then)
     also
-    have "and_then x (Fstack S) \<sqsubseteq> FTree.single x \<otimes>\<otimes> Fstack S" by (rule and_then_both_single')
+    have "and_then x (Fstack as S) \<sqsubseteq> single x \<otimes>\<otimes> Fstack as S" by (rule and_then_both_single')
     note pathsCard_mono'[OF paths_mono[OF substitute_mono2'[OF this]]]
     also
-    have "FTree.single x \<sqsubseteq> Fexp (Var x)\<cdot>a" by (rule Fexp_Var)
+    have "single x \<sqsubseteq> Fexp (Var x)\<cdot>a" by (rule Fexp_Var)
     note pathsCard_mono'[OF paths_mono[OF substitute_mono2'[OF both_mono1'[OF this]]]]
     finally
-    have "pathsCard (paths (substitute (FBinds \<Gamma>\<cdot>ae) (thunks \<Gamma>) (Fexp e\<cdot>u  \<otimes>\<otimes> Fstack S))) \<sqsubseteq> record_call x\<cdot>(pathsCard (paths (substitute (FBinds \<Gamma>\<cdot>ae) (thunks \<Gamma>) (Fexp (Var x)\<cdot>a  \<otimes>\<otimes> Fstack S))))" 
+    have "pathsCard (paths (substitute (FBinds \<Gamma>\<cdot>ae) (thunks \<Gamma>) (Fexp e\<cdot>u  \<otimes>\<otimes> Fstack as S))) \<sqsubseteq> record_call x\<cdot>(pathsCard (paths (substitute (FBinds \<Gamma>\<cdot>ae) (thunks \<Gamma>) (Fexp (Var x)\<cdot>a \<otimes>\<otimes> Fstack as S))))" 
       by this simp_all
-    thus "prognosis ae u (\<Gamma>, e, S) \<sqsubseteq> record_call x\<cdot>(prognosis ae a (\<Gamma>, Var x, S))" by simp
+    thus "prognosis ae as u (\<Gamma>, e, S) \<sqsubseteq> record_call x\<cdot>(prognosis ae as a (\<Gamma>, Var x, S))" by simp
   next
-    fix \<Gamma> :: heap and e :: exp and x :: var and ae :: AEnv and u a S
+    fix \<Gamma> :: heap and e :: exp and x :: var and ae :: AEnv and as u a S
     assume "map_of \<Gamma> x = Some e"
     assume "ae x = up\<cdot>u"
     assume "\<not> isVal e"
@@ -159,36 +157,36 @@ begin
     hence [simp]: "f_nxt (FBinds \<Gamma>\<cdot>ae) (thunks \<Gamma>) x = FBinds (delete x \<Gamma>)\<cdot>ae" 
       by (auto simp add: f_nxt_def Fexp.AnalBinds_delete_to_fun_upd empty_is_bottom)
 
-    have "pathsCard (paths (substitute (FBinds (delete x \<Gamma>)\<cdot>ae) (thunks (delete x \<Gamma>)) (Fexp e\<cdot>u \<otimes>\<otimes> Fstack S)))
-       =  pathsCard (paths (substitute (FBinds (delete x \<Gamma>)\<cdot>ae) (thunks \<Gamma>) (Fexp e\<cdot>u \<otimes>\<otimes> Fstack S)))"
+    have "pathsCard (paths (substitute (FBinds (delete x \<Gamma>)\<cdot>ae) (thunks (delete x \<Gamma>)) (Fexp e\<cdot>u \<otimes>\<otimes> Fstack as S)))
+       =  pathsCard (paths (substitute (FBinds (delete x \<Gamma>)\<cdot>ae) (thunks \<Gamma>) (Fexp e\<cdot>u \<otimes>\<otimes> Fstack as S)))"
        by (rule arg_cong[OF substitute_cong_T]) (auto simp add: empty_is_bottom)
-    also have "\<dots>  = pathsCard (paths (nxt (and_then x (substitute (FBinds (delete x \<Gamma>)\<cdot>ae) (thunks \<Gamma>) (Fexp e\<cdot>u  \<otimes>\<otimes> Fstack S))) x))"
+    also have "\<dots>  = pathsCard (paths (nxt (and_then x (substitute (FBinds (delete x \<Gamma>)\<cdot>ae) (thunks \<Gamma>) (Fexp e\<cdot>u \<otimes>\<otimes> Fstack as S))) x))"
       by simp
     also
-    have "\<dots> \<sqsubseteq> record_call x\<cdot>(pathsCard (paths (and_then x (substitute (FBinds (delete x \<Gamma>)\<cdot>ae) (thunks \<Gamma>) (Fexp e\<cdot>u  \<otimes>\<otimes> Fstack S)))))"
+    have "\<dots> \<sqsubseteq> record_call x\<cdot>(pathsCard (paths (and_then x (substitute (FBinds (delete x \<Gamma>)\<cdot>ae) (thunks \<Gamma>) (Fexp e\<cdot>u \<otimes>\<otimes> Fstack as S)))))"
       by (rule pathsCard_paths_nxt)
     also
-    have "\<dots> = record_call x\<cdot>(pathsCard (paths (and_then x (substitute (FBinds (delete x \<Gamma>)\<cdot>ae) (thunks \<Gamma>) (Fstack S  \<otimes>\<otimes> Fexp e\<cdot>u)))))"
+    have "\<dots> = record_call x\<cdot>(pathsCard (paths (and_then x (substitute (FBinds (delete x \<Gamma>)\<cdot>ae) (thunks \<Gamma>) (Fstack as S \<otimes>\<otimes> Fexp e\<cdot>u)))))"
       by (metis both_comm)
     also
-    have "\<dots> = record_call x\<cdot>(pathsCard (paths (and_then x (substitute (FBinds (delete x \<Gamma>)\<cdot>ae) (thunks \<Gamma>) (Fstack S  \<otimes>\<otimes> (FBinds \<Gamma>\<cdot>ae) x)))))"
+    have "\<dots> = record_call x\<cdot>(pathsCard (paths (and_then x (substitute (FBinds (delete x \<Gamma>)\<cdot>ae) (thunks \<Gamma>) (Fstack as S \<otimes>\<otimes> (FBinds \<Gamma>\<cdot>ae) x)))))"
       using `map_of \<Gamma> x = Some e` `ae x = up\<cdot>u` by (simp add: Fexp.AnalBinds_lookup)
     also
-    have "and_then x (substitute (FBinds (delete x \<Gamma>)\<cdot>ae) (thunks \<Gamma>) (Fstack S \<otimes>\<otimes> (FBinds \<Gamma>\<cdot>ae) x)) = substitute (FBinds \<Gamma>\<cdot>ae) (thunks \<Gamma>) (and_then x (Fstack S))"
+    have "and_then x (substitute (FBinds (delete x \<Gamma>)\<cdot>ae) (thunks \<Gamma>) (Fstack as S \<otimes>\<otimes> (FBinds \<Gamma>\<cdot>ae) x)) = substitute (FBinds \<Gamma>\<cdot>ae) (thunks \<Gamma>) (and_then x (Fstack as S))"
       by (simp add: substitute_and_then)
     also
-    have "and_then x (Fstack S) \<sqsubseteq> FTree.single x \<otimes>\<otimes> Fstack S" by (rule and_then_both_single')
+    have "and_then x (Fstack as S) \<sqsubseteq> single x \<otimes>\<otimes> Fstack as S" by (rule and_then_both_single')
     note pathsCard_mono'[OF paths_mono[OF substitute_mono2'[OF this]]]
     also
-    have "FTree.single x \<sqsubseteq> Fexp (Var x)\<cdot>a" by (rule Fexp_Var)
+    have "single x \<sqsubseteq> Fexp (Var x)\<cdot>a" by (rule Fexp_Var)
     note pathsCard_mono'[OF paths_mono[OF substitute_mono2'[OF both_mono1'[OF this]]]]
     finally
-    have "pathsCard (paths (substitute (FBinds (delete x \<Gamma>)\<cdot>ae) (thunks (delete x \<Gamma>)) (Fexp e\<cdot>u  \<otimes>\<otimes> Fstack S)))
-       \<sqsubseteq> record_call x\<cdot>(pathsCard (paths (substitute (FBinds \<Gamma>\<cdot>ae) (thunks \<Gamma>) (Fexp (Var x)\<cdot>a  \<otimes>\<otimes> Fstack S))))" 
+    have "pathsCard (paths (substitute (FBinds (delete x \<Gamma>)\<cdot>ae) (thunks (delete x \<Gamma>)) (Fexp e\<cdot>u  \<otimes>\<otimes> Fstack as S)))
+       \<sqsubseteq> record_call x\<cdot>(pathsCard (paths (substitute (FBinds \<Gamma>\<cdot>ae) (thunks \<Gamma>) (Fexp (Var x)\<cdot>a  \<otimes>\<otimes> Fstack as S))))" 
       by this simp_all
-    thus "prognosis ae u (delete x \<Gamma>, e, Upd x # S) \<sqsubseteq> record_call x\<cdot>(prognosis ae a (\<Gamma>, Var x, S))" by simp
+    thus "prognosis ae as u (delete x \<Gamma>, e, Upd x # S) \<sqsubseteq> record_call x\<cdot>(prognosis ae as a (\<Gamma>, Var x, S))" by simp
   next
-    fix \<Gamma> :: heap and e :: exp and ae :: AEnv and  x :: var and  S
+    fix \<Gamma> :: heap and e :: exp and ae :: AEnv and  x :: var and as S
     assume "isVal e"
     hence "repeatable (Fexp e\<cdot>0)" by (rule Fun_repeatable)
 
@@ -199,16 +197,36 @@ begin
       by (auto simp add: thunks_Cons dest: set_mp[OF thunks_domA])
 
     have "fup\<cdot>(Fexp e)\<cdot>(ae x) \<sqsubseteq> Fexp e\<cdot>0" by (metis fup2 monofun_cfun_arg up_zero_top)
-    hence "substitute ((FBinds \<Gamma>\<cdot>ae)(x := fup\<cdot>(Fexp e)\<cdot>(ae x))) (thunks \<Gamma>) (Fexp e\<cdot>0 \<otimes>\<otimes> Fstack S) \<sqsubseteq> substitute ((FBinds \<Gamma>\<cdot>ae)(x := Fexp e\<cdot>0)) (thunks \<Gamma>) (Fexp e\<cdot>0 \<otimes>\<otimes> Fstack S)"
+    hence "substitute ((FBinds \<Gamma>\<cdot>ae)(x := fup\<cdot>(Fexp e)\<cdot>(ae x))) (thunks \<Gamma>) (Fexp e\<cdot>0 \<otimes>\<otimes> Fstack as S) \<sqsubseteq> substitute ((FBinds \<Gamma>\<cdot>ae)(x := Fexp e\<cdot>0)) (thunks \<Gamma>) (Fexp e\<cdot>0 \<otimes>\<otimes> Fstack as S)"
       by (intro substitute_mono1' fun_upd_mono below_refl)
-    also have "\<dots> = substitute (((FBinds \<Gamma>\<cdot>ae)(x := Fexp e\<cdot>0))(x := empty)) (thunks \<Gamma>) (Fexp e\<cdot>0 \<otimes>\<otimes> Fstack S)"
+    also have "\<dots> = substitute (((FBinds \<Gamma>\<cdot>ae)(x := Fexp e\<cdot>0))(x := empty)) (thunks \<Gamma>) (Fexp e\<cdot>0 \<otimes>\<otimes> Fstack as S)"
       using `repeatable (Fexp e\<cdot>0)` by (rule substitute_remove_anyways, simp)
     also have "((FBinds \<Gamma>\<cdot>ae)(x := Fexp e\<cdot>0))(x := empty) = FBinds \<Gamma>\<cdot>ae"
       by (simp add: fun_upd_idem Fexp.AnalBinds_not_there empty_is_bottom)
     finally
-    show "prognosis ae 0 ((x, e) # \<Gamma>, e, S) \<sqsubseteq> prognosis ae 0 (\<Gamma>, e, Upd x # S)"
+    show "prognosis ae as 0 ((x, e) # \<Gamma>, e, S) \<sqsubseteq> prognosis ae as 0 (\<Gamma>, e, Upd x # S)"
       by (simp, intro pathsCard_mono' paths_mono)
   qed
+
+  sublocale CardinalityPrognosisIfThenElse prognosis
+  proof default
+    fix ae as \<Gamma> scrut e1 e2 S a
+    have "Fexp scrut\<cdot>0 \<otimes>\<otimes> (Fexp e1\<cdot>a \<oplus>\<oplus> Fexp e2\<cdot>a) \<sqsubseteq> Fexp (scrut ? e1 : e2)\<cdot>a"
+      by (rule Fexp_IfThenElse)
+    hence "substitute (FBinds \<Gamma>\<cdot>ae) (thunks \<Gamma>) (Fexp scrut\<cdot>0 \<otimes>\<otimes> (Fexp e1\<cdot>a \<oplus>\<oplus> Fexp e2\<cdot>a) \<otimes>\<otimes> Fstack as S) \<sqsubseteq> substitute (FBinds \<Gamma>\<cdot>ae) (thunks \<Gamma>) (Fexp (scrut ? e1 : e2)\<cdot>a \<otimes>\<otimes> Fstack as S)"
+      by (rule substitute_mono2'[OF both_mono1'])
+    thus "prognosis ae (a#as) 0 (\<Gamma>, scrut, Alts e1 e2 # S) \<sqsubseteq> prognosis ae as a (\<Gamma>, scrut ? e1 : e2, S)"
+      by (simp, intro pathsCard_mono' paths_mono)
+  next
+    fix ae as a \<Gamma> b e1 e2 S
+    have "Fexp (if b then e1 else e2)\<cdot>a \<sqsubseteq> Fexp e1\<cdot>a \<oplus>\<oplus> Fexp e2\<cdot>a"
+      by (auto simp add: either_above_arg1 either_above_arg2)
+    hence "substitute (FBinds \<Gamma>\<cdot>ae) (thunks \<Gamma>) (Fexp (if b then e1 else e2)\<cdot>a \<otimes>\<otimes> Fstack as S) \<sqsubseteq> substitute (FBinds \<Gamma>\<cdot>ae) (thunks \<Gamma>) (Fexp (Bool b)\<cdot>0 \<otimes>\<otimes> (Fexp e1\<cdot>a \<oplus>\<oplus> Fexp e2\<cdot>a) \<otimes>\<otimes> Fstack as S)"
+      by (rule substitute_mono2'[OF both_mono1'[OF below_trans[OF _ both_above_arg2]]])
+    thus "prognosis ae as a (\<Gamma>, if b then e1 else e2, S) \<sqsubseteq> prognosis ae (a#as) 0 (\<Gamma>, Bool b, Alts e1 e2 # S)"
+      by (auto intro!: pathsCard_mono' paths_mono)
+  qed
+
 end
 
 context FTreeAnalysisCardinalityHeap
@@ -242,17 +260,17 @@ begin
 
   sublocale CardinalityPrognosisEdom prognosis 
   proof
-    fix ae a \<Gamma> e S
-    show "edom (prognosis ae a (\<Gamma>, e, S)) \<subseteq> fv \<Gamma> \<union> fv e \<union> fv S"
+    fix ae as a \<Gamma> e S
+    show "edom (prognosis ae as a (\<Gamma>, e, S)) \<subseteq> fv \<Gamma> \<union> fv e \<union> fv S"
       apply (simp add: Union_paths_carrier)
       apply (rule carrier_substitute_below)
-      apply (auto simp add: carrier_Fexp dest: set_mp[OF Aexp_edom] set_mp[OF ap_fv_subset] set_mp[OF carrier_FBinds])
+      apply (auto simp add: carrier_Fexp dest: set_mp[OF Aexp_edom] set_mp[OF carrier_Fstack] set_mp[OF ap_fv_subset] set_mp[OF carrier_FBinds])
       done
   qed
   
   sublocale CardinalityPrognosisLet prognosis cHeap
   proof
-    fix \<Delta> \<Gamma> :: heap and e :: exp and S :: stack and  ae :: AEnv and a :: Arity
+    fix \<Delta> \<Gamma> :: heap and e :: exp and S :: stack and  ae :: AEnv and a :: Arity and as
     assume "atom ` domA \<Delta> \<sharp>* \<Gamma>"
     assume "atom ` domA \<Delta> \<sharp>* S"
     assume "edom ae \<subseteq> domA \<Gamma> \<union> upds S"
@@ -265,9 +283,9 @@ begin
     have const_on1:  "\<And> x. const_on (FBinds \<Delta>\<cdot>(Aheap \<Delta> e\<cdot>a)) (carrier ((FBinds \<Gamma>\<cdot>ae) x)) empty"
       unfolding const_on_edom_disj using fresh_distinct_fv[OF `atom \` domA \<Delta> \<sharp>* \<Gamma>`]
       by (auto dest!: set_mp[OF carrier_FBinds] set_mp[OF Fexp.edom_AnalBinds])
-    have const_on2:  "const_on (FBinds \<Delta>\<cdot>(Aheap \<Delta> e\<cdot>a)) (carrier (Fstack S)) empty"
+    have const_on2:  "const_on (FBinds \<Delta>\<cdot>(Aheap \<Delta> e\<cdot>a)) (carrier (Fstack as S)) empty"
       unfolding const_on_edom_disj using fresh_distinct_fv[OF `atom \` domA \<Delta> \<sharp>* S`]
-      by (auto dest!: set_mp[OF carrier_FBinds] set_mp[OF Fexp.edom_AnalBinds] set_mp[OF ap_fv_subset ])
+      by (auto dest!: set_mp[OF carrier_FBinds] set_mp[OF carrier_Fstack] set_mp[OF Fexp.edom_AnalBinds] set_mp[OF ap_fv_subset ])
     have  const_on3: "const_on (FBinds \<Gamma>\<cdot>ae) (- (- domA \<Delta>)) FTree.empty"
       and const_on4: "const_on (FBinds \<Delta>\<cdot>(Aheap \<Delta> e\<cdot>a)) (domA \<Gamma>) FTree.empty"
       unfolding const_on_edom_disj using fresh_distinct[OF `atom \` domA \<Delta> \<sharp>* \<Gamma>`]
@@ -277,9 +295,9 @@ begin
       using fresh_distinct_fv[OF `atom \` domA \<Delta> \<sharp>* \<Gamma>`]
       by (auto dest: set_mp[OF carrier_FBinds])
     hence disj1': "\<And> x. carrier ((FBinds \<Gamma>\<cdot>ae) x) \<subseteq> - domA \<Delta>" by auto
-    have disj2: "\<And> x. carrier (Fstack S) \<inter> domA \<Delta> = {}"
-      using fresh_distinct_fv[OF `atom \` domA \<Delta> \<sharp>* S`] ap_fv_subset[of S] by auto
-    hence disj2': "carrier (Fstack S) \<subseteq> - domA \<Delta>" by auto
+    have disj2: "\<And> x. carrier (Fstack as S) \<inter> domA \<Delta> = {}"
+      using fresh_distinct_fv[OF `atom \` domA \<Delta> \<sharp>* S`] by (auto dest!: set_mp[OF carrier_Fstack])
+    hence disj2': "carrier (Fstack as S) \<subseteq> - domA \<Delta>" by auto
     
 
     {
@@ -306,8 +324,8 @@ begin
     note FBinds = ext[OF this]
 
     {
-    have "pathsCard (paths (substitute (FBinds (\<Delta> @ \<Gamma>)\<cdot>(Aheap \<Delta> e\<cdot>a \<squnion> ae)) (thunks (\<Delta> @ \<Gamma>)) (Fexp e\<cdot>a \<otimes>\<otimes> Fstack S)))
-      = pathsCard (paths (substitute (FBinds \<Gamma>\<cdot>ae) (thunks (\<Delta> @ \<Gamma>)) (substitute (FBinds \<Delta>\<cdot>(Aheap \<Delta> e\<cdot>a))  (thunks (\<Delta> @ \<Gamma>))  (Fexp e\<cdot>a \<otimes>\<otimes> Fstack S))))"
+    have "pathsCard (paths (substitute (FBinds (\<Delta> @ \<Gamma>)\<cdot>(Aheap \<Delta> e\<cdot>a \<squnion> ae)) (thunks (\<Delta> @ \<Gamma>)) (Fexp e\<cdot>a \<otimes>\<otimes> Fstack as S)))
+      = pathsCard (paths (substitute (FBinds \<Gamma>\<cdot>ae) (thunks (\<Delta> @ \<Gamma>)) (substitute (FBinds \<Delta>\<cdot>(Aheap \<Delta> e\<cdot>a))  (thunks (\<Delta> @ \<Gamma>))  (Fexp e\<cdot>a \<otimes>\<otimes> Fstack as S))))"
        by (simp add: substitute_substitute[OF const_on1] FBinds)
     also have "substitute (FBinds \<Gamma>\<cdot>ae) (thunks (\<Delta> @ \<Gamma>)) = substitute (FBinds \<Gamma>\<cdot>ae) (thunks \<Gamma>)"
       apply (rule substitute_cong_T)
@@ -317,7 +335,7 @@ begin
       apply (rule substitute_cong_T)
       using const_on4
       by (auto dest: set_mp[OF thunks_domA])
-    also have "substitute (FBinds \<Delta>\<cdot>(Aheap \<Delta> e\<cdot>a)) (thunks \<Delta>) (Fexp e\<cdot>a \<otimes>\<otimes> Fstack S) = substitute (FBinds \<Delta>\<cdot>(Aheap \<Delta> e\<cdot>a)) (thunks \<Delta>) (Fexp e\<cdot>a) \<otimes>\<otimes> Fstack S" 
+    also have "substitute (FBinds \<Delta>\<cdot>(Aheap \<Delta> e\<cdot>a)) (thunks \<Delta>) (Fexp e\<cdot>a \<otimes>\<otimes> Fstack as S) = substitute (FBinds \<Delta>\<cdot>(Aheap \<Delta> e\<cdot>a)) (thunks \<Delta>) (Fexp e\<cdot>a) \<otimes>\<otimes> Fstack as S"
       by (rule substitute_only_empty_both[OF const_on2])
     also note calculation
     }
@@ -325,18 +343,18 @@ begin
     also
     note env_restr_split[where S = "domA \<Delta>"]
     also
-    have "pathsCard (paths (substitute (FBinds \<Gamma>\<cdot>ae) (thunks \<Gamma>) (substitute (FBinds \<Delta>\<cdot>(Aheap \<Delta> e\<cdot>a)) (thunks \<Delta>) (Fexp e\<cdot>a) \<otimes>\<otimes> Fstack S))) f|` domA \<Delta> 
+    have "pathsCard (paths (substitute (FBinds \<Gamma>\<cdot>ae) (thunks \<Gamma>) (substitute (FBinds \<Delta>\<cdot>(Aheap \<Delta> e\<cdot>a)) (thunks \<Delta>) (Fexp e\<cdot>a) \<otimes>\<otimes> Fstack as S))) f|` domA \<Delta> 
         = pathsCard (paths (ftree_restr (domA \<Delta>) (substitute (FBinds \<Delta>\<cdot>(Aheap \<Delta> e\<cdot>a)) (thunks \<Delta>) (Fexp e\<cdot>a))))"
           by (simp add: filter_paths_conv_free_restr ftree_restr_both ftree_rest_substitute[OF disj1]  ftree_restr_is_empty[OF disj2])
     also
     have "ftree_restr (domA \<Delta>) (substitute (FBinds \<Delta>\<cdot>(Aheap \<Delta> e\<cdot>a)) (thunks \<Delta>) (Fexp e\<cdot>a)) \<sqsubseteq> Fheap \<Delta> e\<cdot>a"  by (rule Fheap_substitute)
     also
-    have "pathsCard (paths (substitute (FBinds \<Gamma>\<cdot>ae) (thunks \<Gamma>) (substitute (FBinds \<Delta>\<cdot>(Aheap \<Delta> e\<cdot>a)) (thunks \<Delta>) (Fexp e\<cdot>a) \<otimes>\<otimes> Fstack S))) f|` (- domA \<Delta>) =
-          pathsCard (paths (substitute (FBinds \<Gamma>\<cdot>ae) (thunks \<Gamma>) (ftree_restr (- domA \<Delta>) (substitute (FBinds \<Delta>\<cdot>(Aheap \<Delta> e\<cdot>a)) (thunks \<Delta>) (Fexp e\<cdot>a)) \<otimes>\<otimes> Fstack S)))"
+    have "pathsCard (paths (substitute (FBinds \<Gamma>\<cdot>ae) (thunks \<Gamma>) (substitute (FBinds \<Delta>\<cdot>(Aheap \<Delta> e\<cdot>a)) (thunks \<Delta>) (Fexp e\<cdot>a) \<otimes>\<otimes> Fstack as S))) f|` (- domA \<Delta>) =
+          pathsCard (paths (substitute (FBinds \<Gamma>\<cdot>ae) (thunks \<Gamma>) (ftree_restr (- domA \<Delta>) (substitute (FBinds \<Delta>\<cdot>(Aheap \<Delta> e\<cdot>a)) (thunks \<Delta>) (Fexp e\<cdot>a)) \<otimes>\<otimes> Fstack as S)))"
           by (simp add: filter_paths_conv_free_restr2 ftree_rest_substitute2[OF disj1' const_on3] ftree_restr_both  ftree_restr_noop[OF disj2'])
     also have "ftree_restr (- domA \<Delta>) (substitute (FBinds \<Delta>\<cdot>(Aheap \<Delta> e\<cdot>a))  (thunks \<Delta>)  (Fexp e\<cdot>a)) \<sqsubseteq> Fexp (Terms.Let \<Delta> e)\<cdot>a" by (rule Fexp_Let)
     finally
-    show "prognosis (Aheap \<Delta> e\<cdot>a \<squnion> ae) a (\<Delta> @ \<Gamma>, e, S) \<sqsubseteq> cHeap \<Delta> e\<cdot>a \<squnion> prognosis ae a (\<Gamma>, Terms.Let \<Delta> e, S)"
+    show "prognosis (Aheap \<Delta> e\<cdot>a \<squnion> ae) as a (\<Delta> @ \<Gamma>, e, S) \<sqsubseteq> cHeap \<Delta> e\<cdot>a \<squnion> prognosis ae as a (\<Gamma>, Terms.Let \<Delta> e, S)"
       by (simp add: cHeap_def del: fun_meet_simp) 
   qed
 
